% vim:ft=tex

\paragraph{Problem}

Find the Laplace transform of the following function
$$
	f(t)=\begin{cases}
		e^{4t} & \text{if } 0<t<5 \\
		1      & \text{if } t>5
	\end{cases}
$$

\paragraph{Solution}

\def\L{\mathcal L}
\def\LI{\mathcal L^{-1}}

By inspection:
$$
	f(t)=u_0(t)(e^{4t}-1) - u_5(t)(e^{4t}-1) + 1
$$
(Draw a graph to convince yourself.)

Manipulating, we get
\begin{align*}
	f(t) & = u_0(t)(e^{4t}) - u_5(t)(e^{4t}) - u_0(t) - u_5(t) + 1           \\
	     & = u_0(t)(e^{4t}) - u_5(t)(e^{4(t-5)}e^{20}) - u_0(t) - u_5(t) + 1 \\
	     & = u_0(t)(e^{4t}) - e^{20}u_5(t)(e^{4(t-5)}) - u_0(t) - u_5(t) + 1
\end{align*}

Next, let's pre-process some Laplace transforms as building blocks:
\begin{align*}
	\L(e^{4t})           & =\frac1{s-4}          \\
	\L(u(t-c)e^{4(t-c)}) & = \frac{e^{-cs}}{s-4} \\
	\L(u(t)e^{4t})       & = \frac1{s-4}         \\
	\L(u_5(t)e^{4(t-5)}) & = \frac{e^{-5s}}{s-4} \\
	\L(u_0)              & = \frac1s             \\
	\L(u_5)              & = \frac{e^{-5s}}s     \\
	\L(1)                & = \frac1s
\end{align*}

So then
\begin{align*}
	\L(f) & =\frac1{s-4}-e^{20}\frac{e^{-5s}}{s-4}-\frac1s-\frac{e^{-5s}}s+\frac1s \\
	      & =\frac1{s-4}-e^{20}\frac{e^{-5s}}{s-4}-\frac{e^{-5s}}s                 \\
	% & =1/(s-4)-e^(20-5s)/(s-4)-(e^(-5s))/s                 \\
\end{align*}

\newpage\paragraph{Problem}
Let
$$
	g(t):=\begin{cases}
		t    & \text{if }t\leq4\pi \\
		4\pi & \text{if }t>4\pi
	\end{cases}
$$
Solve the differential equation
$$
	y'' + 16y = g(t),\Quad y(0)=6,y'(0)=5
$$
using Laplace transforms.
$$
	y=\begin{cases}
		? & \text{if }t\leq4\pi \\
		? & \text{if }t>4\pi
	\end{cases}
$$

\paragraph{Solution}

First, we write $g(t)$ in terms of a step function.
$$
	g(t) = t - u(t-4\pi)(t-4\pi)
$$
Then, we pre-process some Laplace transforms.
\begin{align*}
	\L(t)                   & = \frac1{s^2}             \\
	\L(u_{4\pi}(t)(t-4\pi)) & = e^{-4\pi s}\L(t)        \\
	                        & = \frac{e^{-4\pi s}}{s^2}
\end{align*}
And now for $Y(s):=\L(y)$;
\begin{alignat*}{2}
	\L(y')  & = -y(0)+sY(s)    &  & = -6+sY(s)      \\
	\L(y'') & = -y'(0)+s\L(y') &  & = -5-6s+s^2Y(s) \\
\end{alignat*}

Applying the Laplace transform on the entire differential equation:
\begin{align*}
	-5-6s+s^2Y(s)+16Y(s) & = \frac1{s^2}-\frac{e^{-4\pi s}}{s^2}                                 \\
	(s^2+16)Y(s)         & = \frac{1-e^{-4\pi s}}{s^2}+6s+5                                      \\
	Y(s)                 & = \frac{1-e^{-4\pi s}}{(s^2)(s^2+16)}+\frac{6s+5}{s^2+16}\tag*{($*$)}
\end{align*}
Breaking into a sub-problem:
\begin{align*}
	Y_1(s)      & =\frac1{(s^2)(s^2+16)}                                      \\
	            & =\frac{1}{16s^2}-\frac{1}{16(s^2+16)}                       \\
	Y_1(s)      & =\frac{1}{16}\left(\frac{1}{s^2}-\frac{1}{s^2+16}\right)    \\
	\LI(Y_1(s)) & =\frac{1}{16}\left(t-\frac{\sin(4t)}{4}\right)\tag*{($**$)}
\end{align*}
And another sub-problem:
\begin{align*}
	Y_2(s)      & =\frac{e^{-4\pi s}}{(s^2)(s^2+16)}                                                                                     \\
	Y_2(s)      & =\frac{1}{16}\left(\frac{e^{-4\pi s}}{s^2}-\frac{e^{-4\pi s}}{s^2+16}\right)                                           \\
	\LI(Y_2(s)) & \stackrel{\text{\hyperref[c8f0f6e]{R1}}}{=}\frac{1}{16}\left(u_{4\pi}(t)(t-4\pi)-\frac{u_{4\pi}(t)\sin(4t)}{4}\right) \\
	            & =\frac{u_{4\pi}(t)}{16}\left(t-4\pi-\frac{\sin(4t)}{4}\right)\tag*{($***$)}
\end{align*}
Finally, using $(**)$ and $(***)$ on $(*)$, we have
\begin{align*}
	\LI(Y(s))
	 & = -\frac{u_{4\pi}(t)}{16}\left(t-4\pi-\frac{\sin(4t)}{4}\right)+
	\frac{1}{16}\left(t-\frac{\sin(4t)}{4}\right)+
	\frac54\sin(4t)+6\cos(4t)                                           \\
	 & = \frac{u_{4\pi}(t)}{16}\left(-t+4\pi+\frac{\sin(4t)}{4}\right)+
	\frac{1}{16}\left(t+\frac{79\sin(4t)}{4}+96\cos(4t)\right)
\end{align*}

To the left of $t=4\pi$, the step function $u_{4\pi}(t)$ evaluates to
zero, and we have
$$
	\LI(Y(s))=\frac{1}{16}\left(t+\frac{79\sin(4t)}{4}+96\cos(4t)\right)
$$
and to its right we have
\begin{align*}
	\LI(Y(s))
	 & = \frac{1}{16}\left(-t+4\pi+\frac{\sin(4t)}{4}\right)+
	\frac{1}{16}\left(t+\frac{79\sin(4t)}{4}+96\cos(4t)\right) \\
	 & =\frac{1}{16}\big[4\pi+20\sin(4t)+96\cos(4t)\big]       \\
	%(1/16)(t+(79/4)sin(4t)+96cos(4t))
	%(1/16)(4pi+20sin(4t)+96cos(4t))
\end{align*}

\Result{1}{}\label{c8f0f6e}

Let $f(t):=\frac14\sin(4t)$. Then $F(s)=\frac1{s^2+16}$, and
$$
	\L(u(t-4\pi)f(t-4\pi))=e^{-4\pi s}F(s)
$$
However, since $f(t-4\pi)=f(t)$, we have
$$
	\L(u(t-4\pi)f(t-4\pi))=\L(u(t-4\pi)f(t))
$$
and hence
$$
	\LI\left(\frac{e^{-4\pi s}}{s^2+16}\right)=u(t-4\pi)f(t) = u_{4\pi}(t)f(t)
$$
